pulse/lib/common/Pulse.Lib.Core.fsti
@@ -1041,8 +1041,6 @@ let no_extrude (p: slprop) : slprop = p
 
 let old () = ()
 
-let _rec_knot = ()
-
 let rewrites_to_p #t (x y: t) = (x == y)
 
 (*
