pulse/lib/pulse/lib/Pulse.Lib.WhileLoop.fst
@@ -24,7 +24,7 @@ fn rec while_loop'
   (inv:bool -> slprop)
   (cond:unit -> stt bool (exists* x. inv x) (fun b -> inv b))
   (body:unit -> stt unit (inv true) (fun _ -> exists* x. inv x))
-  requires (exists* x. inv x)
+  requires no_extrude (exists* x. inv x)
   ensures inv false
 {
   let b = cond ();
